examples/nsl_pk_no_events_lookup/DY.Example.NSL.Protocol.Stateful.fst
@@ -15,9 +15,9 @@ open DY.Example.NSL.Protocol.Total
 
 [@@ with_bytes bytes]
 type nsl_session =
-  | InitiatorSentMsg1: b:principal -> n_a:bytes -> nsl_session
-  | ResponderSentMsg2: a:principal -> n_a:bytes -> n_b:bytes -> nsl_session
-  | InitiatorSentMsg3: b:principal -> n_a:bytes -> n_b:bytes -> nsl_session
+  | InitiatorSendingMsg1: b:principal -> n_a:bytes -> nsl_session
+  | ResponderSendingMsg2: a:principal -> n_a:bytes -> n_b:bytes -> nsl_session
+  | InitiatorSendingMsg3: b:principal -> n_a:bytes -> n_b:bytes -> nsl_session
   | ResponderReceivedMsg3: a:principal -> n_a:bytes -> n_b:bytes -> nsl_session
 
 %splice [ps_nsl_session] (gen_parser (`nsl_session))
@@ -39,7 +39,7 @@ instance local_state_nsl_session: local_state nsl_session = {
 
 [@@ with_bytes bytes]
 type nsl_event =
-  | Respond1: a:principal -> b:principal -> n_a:bytes -> n_b:bytes -> nsl_event
+  | Responding: a:principal -> b:principal -> n_a:bytes -> n_b:bytes -> nsl_event
 
 %splice [ps_nsl_event] (gen_parser (`nsl_event))
 %splice [ps_nsl_event_is_well_formed] (gen_is_well_formed_lemma (`nsl_event))
@@ -61,14 +61,14 @@ val prepare_msg1: principal -> principal -> traceful state_id
 let prepare_msg1 alice bob =
   let* n_a = mk_rand NoUsage (join (principal_label alice) (principal_label bob)) 32 in
   let* sess_id = new_session_id alice in
-  set_state alice sess_id (InitiatorSentMsg1 bob n_a <: nsl_session);*
+  set_state alice sess_id (InitiatorSendingMsg1 bob n_a <: nsl_session);*
   return sess_id
 
 val send_msg1: nsl_global_sess_ids -> principal -> state_id -> traceful (option timestamp)
 let send_msg1 global_sess_id alice sess_id =
   let*? st = get_state alice sess_id in
-  guard_tr (InitiatorSentMsg1? st);*?
-  let InitiatorSentMsg1 bob n_a = st in
+  guard_tr (InitiatorSendingMsg1? st);*?
+  let InitiatorSendingMsg1 bob n_a = st in
   let*? pk_b = get_public_key alice global_sess_id.pki (PkEnc "NSL.PublicKey") bob in
   let* nonce = mk_rand PkNonce (principal_label alice) 32 in
   let msg = compute_message1 alice bob pk_b n_a nonce in
@@ -80,7 +80,7 @@ let send_msg1_ global_sess_id alice bob =
   let* n_a = mk_rand NoUsage (join (principal_label alice) (principal_label bob)) 32 in
 
   let* sess_id = new_session_id alice in
-  let st = InitiatorSentMsg1 bob n_a in
+  let st = InitiatorSendingMsg1 bob n_a in
   set_state alice sess_id st;*
 
   let*? pk_b = get_public_key alice global_sess_id.pki (PkEnc "NSL.PublicKey") bob in
@@ -97,16 +97,16 @@ let prepare_msg2 global_sess_id bob msg_id =
   let*? sk_b = get_private_key bob global_sess_id.private_keys (PkDec "NSL.PublicKey") in
   let*? msg1: message1 = return (decode_message1 bob msg sk_b) in
   let* n_b = mk_rand NoUsage (join (principal_label msg1.alice) (principal_label bob)) 32 in
-  trigger_event bob (Respond1 msg1.alice bob msg1.n_a n_b);*
+  trigger_event bob (Responding msg1.alice bob msg1.n_a n_b);*
   let* sess_id = new_session_id bob in
-  set_state bob sess_id (ResponderSentMsg2 msg1.alice msg1.n_a n_b <: nsl_session);*
+  set_state bob sess_id (ResponderSendingMsg2 msg1.alice msg1.n_a n_b <: nsl_session);*
   return (Some sess_id)
 
 val send_msg2: nsl_global_sess_ids -> principal -> state_id -> traceful (option timestamp)
 let send_msg2 global_sess_id bob sess_id =
   let*? st = get_state bob sess_id in
-  guard_tr (ResponderSentMsg2? st);*?
-  let ResponderSentMsg2 alice n_a n_b = st in
+  guard_tr (ResponderSendingMsg2? st);*?
+  let ResponderSendingMsg2 alice n_a n_b = st in
   let*? pk_a = get_public_key bob global_sess_id.pki (PkEnc "NSL.PublicKey") alice in
   let* nonce = mk_rand PkNonce (principal_label bob) 32 in
   let msg = compute_message2 bob {n_a; alice;} pk_a n_b nonce in
@@ -123,9 +123,9 @@ let send_msg2_ global_sess_id bob msg_id =
   let alice = msg1.alice in
   let n_a = msg1.n_a in
   let* n_b = mk_rand NoUsage (join (principal_label alice) (principal_label bob)) 32 in
-  trigger_event bob (Respond1 alice bob n_a n_b);*
+  trigger_event bob (Responding alice bob n_a n_b);*
   
-  let st = ResponderSentMsg2 alice n_a n_b in
+  let st = ResponderSendingMsg2 alice n_a n_b in
   let* sess_id = new_session_id bob in
   set_state bob sess_id st;*
   
@@ -142,10 +142,10 @@ let prepare_msg3 global_sess_id alice sess_id msg_id =
   let*? msg = recv_msg msg_id in
   let*? sk_a = get_private_key alice global_sess_id.private_keys (PkDec "NSL.PublicKey") in
   let*? st = get_state alice sess_id in
-  guard_tr (InitiatorSentMsg1? st);*?
-  let InitiatorSentMsg1 bob n_a = st in
+  guard_tr (InitiatorSendingMsg1? st);*?
+  let InitiatorSendingMsg1 bob n_a = st in
   let*? msg2: message2 = return (decode_message2 alice bob msg sk_a n_a) in
-  set_state alice sess_id (InitiatorSentMsg3 bob n_a msg2.n_b <: nsl_session);*
+  set_state alice sess_id (InitiatorSendingMsg3 bob n_a msg2.n_b <: nsl_session);*
   return (Some ())
 
 val prepare_msg3_: nsl_global_sess_ids -> principal -> timestamp -> traceful (option state_id)
@@ -154,16 +154,16 @@ let prepare_msg3_ global_sess_id alice msg_id =
   let*? sk_a = get_private_key alice global_sess_id.private_keys (PkDec "NSL.PublicKey") in
   let*? msg2: message2 = return (decode_message2_ alice msg sk_a) in
   let p = (fun (s:nsl_session) -> 
-    (InitiatorSentMsg1? s) && 
-    (InitiatorSentMsg1?.n_a s = msg2.n_a) && 
-    (InitiatorSentMsg1?.b s = msg2.bob))  in
+    (InitiatorSendingMsg1? s) && 
+    (InitiatorSendingMsg1?.n_a s = msg2.n_a) && 
+    (InitiatorSendingMsg1?.b s = msg2.bob))  in
   let* tr = get_trace in
   let (opt_st, _) = lookup_state #nsl_session alice p tr in
   match opt_st with
   | None -> return None
   | Some (st, sid ) -> (
-      let InitiatorSentMsg1 bob n_a = st in
-      set_state alice sid (InitiatorSentMsg3 bob n_a msg2.n_b <: nsl_session);*
+      let InitiatorSendingMsg1 bob n_a = st in
+      set_state alice sid (InitiatorSendingMsg3 bob n_a msg2.n_b <: nsl_session);*
       return (Some sid)
   )
 
@@ -171,8 +171,8 @@ let prepare_msg3_ global_sess_id alice msg_id =
 val send_msg3: nsl_global_sess_ids -> principal -> state_id -> traceful (option timestamp)
 let send_msg3 global_sess_id alice sess_id =
   let*? st = get_state alice sess_id in
-  guard_tr (InitiatorSentMsg3? st);*?
-  let InitiatorSentMsg3 bob n_a n_b = st in
+  guard_tr (InitiatorSendingMsg3? st);*?
+  let InitiatorSendingMsg3 bob n_a n_b = st in
   let*? pk_b = get_public_key alice global_sess_id.pki (PkEnc "NSL.PublicKey") bob in
   let* nonce = mk_rand PkNonce (principal_label alice) 32 in
   let msg = compute_message3 alice bob pk_b n_b nonce in
@@ -186,17 +186,17 @@ let send_msg3_ global_sess_id alice msg_id =
   let*? msg2: message2 = return (decode_message2_ alice msg sk_a) in
   
   let p = (fun (s:nsl_session) -> 
-    (InitiatorSentMsg1? s) && 
-    (InitiatorSentMsg1?.n_a s = msg2.n_a) && 
-    (InitiatorSentMsg1?.b s = msg2.bob))  in
+    (InitiatorSendingMsg1? s) && 
+    (InitiatorSendingMsg1?.n_a s = msg2.n_a) && 
+    (InitiatorSendingMsg1?.b s = msg2.bob))  in
   let* tr = get_trace in
   let (opt_st, _) = lookup_state #nsl_session alice p tr in
   match opt_st with
   | None -> return None
   | Some (st, sid ) -> (
       let n_b = msg2.n_b in
-      let InitiatorSentMsg1 bob n_a = st in
-      let st = InitiatorSentMsg3 bob n_a n_b in
+      let InitiatorSendingMsg1 bob n_a = st in
+      let st = InitiatorSendingMsg3 bob n_a n_b in
       set_state alice sid st;*
   
   let*? pk_b = get_public_key alice global_sess_id.pki (PkEnc "NSL.PublicKey") bob in
@@ -211,8 +211,8 @@ let prepare_msg4 global_sess_id bob sess_id msg_id =
   let*? msg = recv_msg msg_id in
   let*? sk_b = get_private_key bob global_sess_id.private_keys (PkDec "NSL.PublicKey") in
   let*? st = get_state bob sess_id in
-  guard_tr (ResponderSentMsg2? st);*?
-  let ResponderSentMsg2 alice n_a n_b = st in
+  guard_tr (ResponderSendingMsg2? st);*?
+  let ResponderSendingMsg2 alice n_a n_b = st in
   let*? msg3: message3 = return (decode_message3 alice bob msg sk_b n_b) in
   set_state bob sess_id (ResponderReceivedMsg3 alice n_a n_b <: nsl_session);*
   return (Some ())
@@ -224,14 +224,14 @@ let receive_msg3 global_sess_id bob msg_id =
 
   let*? msg3: message3 = return (decode_message3_ msg sk_b) in
   let p = (fun (s:nsl_session) -> 
-    (ResponderSentMsg2? s) && 
-    (ResponderSentMsg2?.n_b s = msg3.n_b)) in
+    (ResponderSendingMsg2? s) && 
+    (ResponderSendingMsg2?.n_b s = msg3.n_b)) in
   let* tr = get_trace in
   let (opt_st, _) = lookup_state #nsl_session bob p tr in
   match opt_st with
   | None -> return None
   | Some (st, sid ) -> (
-         let ResponderSentMsg2 alice n_a n_b = st in
+         let ResponderSendingMsg2 alice n_a n_b = st in
          set_state bob sid (ResponderReceivedMsg3 alice n_a n_b <: nsl_session);*
   return (Some ())
   )
